\documentclass[a4paper,10pt]{article}

\begin{document}

Firstly, we write expressions for the values of the bits of each node in terms of the
values of those nodes' children.\

$V_{1,1} = \bigwedge\limits_{i=1}^3V_{1i,1}$\

$V_{1,2} = \bigwedge\limits_{i=1}^3\left(V_{1i,2} \vee \left(V_{1i,1} \oplus V_{1,1}\right) \right)$\

$V_{1,3} = \bigwedge\limits_{i=1}^3\left(V_{1i,3} \vee \left(V_{1i,2} \oplus V_{1,2}\right) \vee \left(V_{1i,1} \oplus V_{1,1}\right) \right)$\

\hfill\break

$V_{1i,1} = \bigvee\limits_{j=1}^3 V_{1ij,1}$\

$V_{1i,2} = \bigvee\limits_{j	=1}^3\left(V_{1ij,2} \wedge \neg \left(V_{1ij,1} \oplus V_{1i,1}\right) \right)$\

$V_{1i,3} = \bigvee\limits_{j=1}^3\left(V_{1ij,3} \wedge \neg \left(V_{1ij,2} \oplus V_{1i,2}\right) \wedge \neg \left(V_{1ij,1} \oplus V_{1i,1}\right) \right)$\

\hfill\break

$V_{1ij,1} = \bigwedge\limits_{k=1}^3V_{1ijk,1}$\

$V_{1ij,2} = \bigwedge\limits_{k=1}^3\left(V_{1ijk,2} \vee \left(V_{1ijk,1} \oplus V_{1ij,1}\right) \right)$\

$V_{1ij,3} = \bigwedge\limits_{k=1}^3\left(V_{1ijk,3} \vee \left(V_{1ijk,2} \oplus V_{1ij,2}\right) \vee \left(V_{1ijk,1} \oplus V_{1ij,1}\right) \right)$\


\hfill\break
\hfill\break

Next, we change our equations to propositional logic biconditionals, and conjunct all of our terms
together.   This gives us a single true expression to convert to CNF.\

$V_{1,1} \leftrightarrow \bigwedge\limits_{i=1}^3V_{1i,1} \wedge $\

$V_{1,2} \leftrightarrow \bigwedge\limits_{i=1}^3\left(V_{1i,2} \vee \left(V_{1i,1} \oplus V_{1,1}\right) \right) \wedge $\

$V_{1,3} \leftrightarrow \bigwedge\limits_{i=1}^3\left(V_{1i,3} \vee \left(V_{1i,2} \oplus V_{1,2}\right) \vee \left(V_{1i,1} \oplus V_{1,1}\right) \right) \wedge $\


$V_{1i,1} \leftrightarrow \bigvee\limits_{j=1}^3 V_{1ij,1} \wedge $\

$V_{1i,2} \leftrightarrow \bigvee\limits_{j	=1}^3\left(V_{1ij,2} \wedge \neg \left(V_{1ij,1} \oplus V_{1i,1}\right) \right) \wedge$\

$V_{1i,3} \leftrightarrow \bigvee\limits_{j=1}^3\left(V_{1ij,3} \wedge \neg \left(V_{1ij,2} \oplus V_{1i,2}\right) \wedge \neg \left(V_{1ij,1} \oplus V_{1i,1}\right) \right) \wedge $\


$V_{1ij,1} \leftrightarrow \bigwedge\limits_{k=1}^3V_{1ijk,1} \wedge $\

$V_{1ij,2} \leftrightarrow \bigwedge\limits_{k=1}^3\left(V_{1ijk,2} \vee \left(V_{1ijk,1} \oplus V_{1ij,1}\right) \right) \wedge $\

$V_{1ij,3} \leftrightarrow \bigwedge\limits_{k=1}^3\left(V_{1ijk,3} \vee \left(V_{1ijk,2} \oplus V_{1ij,2}\right) \vee \left(V_{1ijk,1} \oplus V_{1ij,1}\right) \right)$\


\hfill\break

Now, we begin simplifying each term of our massive conjunction to CNF, so that our whole expression
will end up in CNF.\

We do this by writing everything in terms of conjunctions, disjunctions, and negations, then distribute as
necessary until we find ourselves in CNF.
\

\hfill\break

$\left( \bigwedge\limits_{i=1}^3 \left(V_{1i,1} \vee \neg V_{1,1}\right) \right) \wedge \left(V_{1,1} \vee \bigvee\limits_{i=1}^3 \neg V_{1i,1}\right) \wedge$\

$\bigwedge \limits_{i=1}^3 \left( \left( \neg V_{1,2} \vee V_{1i,2} \vee V_{1,1} \vee V{1i,1} \right) \wedge \left( \neg V_{1,2} \vee V_{1i,2} \vee \neg V_{1,1} \vee \neg V{1i,1} \right) \right) \wedge$\

$\bigwedge \limits_{s \in \{1,2,3,4\}^3} \bigvee \limits_{i=1}^3 t_{s_i}$ \\ (where $ t_1 := V_{1,2} \vee \neg V_{1i,2}$, $t_2 := V_{1,2}$, $ t_3 := V_{1,2} \vee V_{1i,1} \vee \neg V_{1,1}$ and $t_4 := V_{1,2} \vee V_{1,1} \vee \neg V_{1i,1}$) \

$\wedge$ \

At this point, we gave up on manually expanding eeverything to CNF,
as about half of the expansions cause the creation of $2^n$ new terms, and
we grew tired of inventing notations in order to fit everything in a sensible
amount of space.  It should be evident that the distributive law can
properly yield the rest of these subexpressions into Conjunctive Normal form.

$\neg V_{1,3} \vee \bigwedge\limits_{i=1}^3\left(V_{1i,3} \vee \left(\left(V_{1i,2} \vee V_{1,2}\right) \wedge \left(\neg V_{1i,2} \vee \neg V_{1,2} \right)\right) \vee \left(\left(V_{1i,1} \vee V_{1,1}\right) \wedge \left(\neg V_{1i,1} \vee \neg V_{1,1}\right) \right) \right) \wedge$\

$V_{1,3} \vee \neg \bigwedge\limits_{i=1}^3\left(V_{1i,3} \vee \left(\left(V_{1i,2} \vee V_{1,2}\right) \wedge \left(\neg V_{1i,2} \vee \neg V_{1,2} \right)\right) \vee \left(\left(V_{1i,1} \vee V_{1,1}\right) \wedge \left(\neg V_{1i,1} \vee \neg V_{1,1}\right) \right) \right) \wedge$\


$V_{1i,1} \vee \neg\bigvee\limits_{j=1}^3 V_{1ij,1} \wedge$\

$\neg V_{1i,1} \vee \bigvee\limits_{j=1}^3 V_{1ij,1} \wedge$\

$V_{1i,2} \vee \neg \bigvee\limits_{j	=1}^3\left(V_{1ij,2} \wedge \left( \left(V_{1ij,1} \wedge V_{1i,1}\right) \vee \left( \neg V_{1ij,1} \wedge \neg V_{1i,1}\right) \right) \right) \wedge$\

$\neg V_{1i,2} \vee  \bigvee\limits_{j	=1}^3\left(V_{1ij,2} \wedge \left( \left(V_{1ij,1} \wedge V_{1i,1}\right) \vee \left( \neg V_{1ij,1} \wedge \neg V_{1i,1}\right) \right) \right) \wedge$\

$V_{1i,3} \vee \neg \bigvee\limits_{j=1}^3\left(V_{1ij,3} \wedge \left( \left(V_{1ij,2} \wedge V_{1i,2}\right) \vee \left(\neg V_{1ij,2} \wedge \neg V_{1i,2}\right) \right) \wedge \left( \left(V_{1ij,1} \wedge V_{1i,1}\right) \vee \left(\neg V_{1ij,1} \wedge \neg V_{1i,1}\right) \right) \right) \wedge$\

$\neg V_{1i,3} \vee \bigvee\limits_{j=1}^3\left(V_{1ij,3} \wedge \left( \left(V_{1ij,2} \wedge V_{1i,2}\right) \vee \left(\neg V_{1ij,2} \wedge \neg V_{1i,2}\right) \right) \wedge \left( \left(V_{1ij,1} \wedge V_{1i,1}\right) \vee \left(\neg V_{1ij,1} \wedge \neg V_{1i,1}\right) \right) \right) \wedge$\

\hfill\break

$\neg V_{1ij,1} \wedge \bigwedge\limits_{k=1}^3V_{1ijk,1} \wedge$\

$V_{1ij,1} \wedge \neg \bigwedge\limits_{k=1}^3V_{1ijk,1} \wedge$\

$V_{1ij,2} \vee \neg \bigwedge\limits_{k=1}^3\left(V_{1ijk,2} \vee \left( \left(V_{1ijk,1} \vee V_{1ij,1}\right) \wedge \left(\neg V_{1ijk,1} \vee \neg V_{1ij,1}\right) \right) \right) \wedge$\

$\neg V_{1ij,2} \vee  \bigwedge\limits_{k=1}^3\left(V_{1ijk,2} \vee \left( \left(V_{1ijk,1} \vee V_{1ij,1}\right) \wedge \left(\neg V_{1ijk,1} \vee \neg V_{1ij,1}\right) \right) \right) \wedge$\

$V_{1ij,3} \vee \neg \bigwedge\limits_{k=1}^3\left(V_{1ijk,3} \vee \left( \left(V_{1ijk,2} \vee V_{1ij,2}\right) \wedge
 \left(\neg V_{1ijk,2} \vee \neg V_{1ij,2}\right) \right) \vee \left( \left(V_{1ijk,1} \vee V_{1ij,1}\right) \wedge \left(\neg V_{1ijk,1} \vee \neg V_{1ij,1}\right) \right) \right) $\

$\wedge$

$\neg V_{1ij,3} \vee \bigwedge\limits_{k=1}^3\left(V_{1ijk,3} \vee \left( \left(V_{1ijk,2} \vee V_{1ij,2}\right) \wedge
 \left(\neg V_{1ijk,2} \vee \neg V_{1ij,2}\right) \right) \vee \left( \left(V_{1ijk,1} \vee V_{1ij,1}\right) \wedge \left(\neg V_{1ijk,1} \vee \neg V_{1ij,1}\right) \right) \right) $



\end{document}
